\documentclass{article}
\usepackage{amsmath}

\begin{document}

\title{Calculus 1 Notes}
\author{}
\date{}

\maketitle

\section{Product Rule}
For functions $f(x)$ and $g(x)$:
\[
\frac{d}{dx}[f(x)g(x)] = f'(x)g(x) + f(x)g'(x)
\]

\section{Quotient Rule}
For functions $f(x)$ and $g(x)$:
\[
	\frac{d}{dx}\left(\frac{f(x)}{g(x)}\right) = \frac{f'(x)g(x)-f(x)g'(x)}{(g(x))^2}
\]

\section{Chain Rule}
For a composite function $f(g(x))$:
\[
\frac{d}{dx}[f(g(x))] = f'(g(x)) \cdot g'(x)
\]
And
\[
\frac{dy}{dx}=\frac{dy}{du}\frac{du}{dx}
\]

\section{Common Derivatives}

\subsection{Natural Logarithm}
\[
\frac{d}{dx}[\ln(x)] = \frac{1}{x}, \quad x > 0
\]

\subsection{Logarithm Base a}
\[
\frac{d}{dx}[\log_{a}(x)] = \frac{1}{x \ln(a)}, \quad x > 0
\]

\subsection{Sine}
\[
\frac{d}{dx}[\sin(x)] = \cos(x)
\]

\subsection{Cosine}
\[
\frac{d}{dx}[\cos(x)] = -\sin(x)
\]

\end{document}
